src/SlabsCommon.fsti
@@ -107,6 +107,8 @@ let lemma_partition_and_pred_implies_mem3
     Classical.move_requires (ALG.lemma_mem_implies_pred pred3 hd3 s) idx;
     Classical.move_requires (ALG.lemma_mem_implies_pred pred4 hd4 s) idx
 
+open Guards
+
 unfold
 let blob
   = slab_metadata &
@@ -139,7 +141,7 @@ let p_guard (size_class) : blob -> vprop
   fun (b:blob) ->
     slab_vprop size_class (snd b) (fst b)
     `VR2.vrefine`
-    (fun ((|s,_|), _) -> is_guard size_class (snd b))
+    (is_guard size_class (snd b) (fst b))
 
 val p_empty_unpack (#opened:_)
   (sc: sc)
@@ -211,9 +213,8 @@ val p_guard_unpack (#opened:_)
     let blob1
       : t_of (slab_vprop sc (snd b2) (fst b2))
       = h1 (slab_vprop sc (snd b2) (fst b2)) in
-    let v1 : Seq.lseq U64.t 4 = dfst (fst blob1) in
     b1 == b2 /\
-    is_guard sc (snd b1) /\
+    is_guard sc (snd b1) (fst b1) blob1 /\
     h0 ((p_guard sc) b1)
     ==
     h1 (slab_vprop sc (snd b2) (fst b2))
@@ -296,8 +297,7 @@ val p_guard_pack (#opened:_)
     let blob0
       : t_of (slab_vprop sc (snd b1) (fst b1))
       = h0 (slab_vprop sc (snd b1) (fst b1)) in
-    let v0 : Seq.lseq U64.t 4 = dfst (fst blob0) in
-    is_guard sc (snd b1) /\
+    is_guard sc (snd b1) (fst b1) blob0 /\
     b1 == b2
   )
   (ensures fun h0 _ h1 ->
@@ -654,7 +654,9 @@ val pack_slab_starseq
       (md_bm_array md_bm_region (US.sizet_to_uint32 idx))) in
     let md : Seq.lseq U64.t 4 = dfst (fst md_blob) in
     //(v == 3ul ==> is_guard size_class md) /\
-    (v == 3ul ==> True) /\
+    (v == 3ul ==> is_guard size_class
+      (slab_array slab_region (US.sizet_to_uint32 idx))
+      (md_bm_array md_bm_region (US.sizet_to_uint32 idx)) md_blob) /\
     (v == 2ul ==> is_full size_class md) /\
     (v == 1ul ==> is_partial size_class md) /\
     (v == 0ul ==> is_empty size_class md) /\
