src/Guards.fsti
@@ -1,6 +1,19 @@
 module Guards
 
 open Utils2
-module U8 = FStar.UInt8
+open SlotsAlloc
 
-val is_guard (size_class: sc) (slab: array U8.t) : prop
+open Steel.Effect
+
+module U8 = FStar.UInt8
+module U32 = FStar.UInt32
+module U64 = FStar.UInt64
+
+module A = Steel.Array
+
+val is_guard
+  (size_class: sc)
+  (arr: array U8.t{A.length arr = U32.v page_size})
+  (md: slab_metadata)
+  (x: normal (t_of (slab_vprop size_class arr md)))
+  : prop
